\begin{filecontents*}{proof.adt}
s($x) divide s($x) = s(zero)
$x ge $x = true
zero ge zero = true

1 – Axiome ligne 25 de Nat.adt
$x ge zero = true
2 – Substitution [zero/$x] dans 1
zero ge zero = true


if s($x) ge s($x) = true then s($x) divide s($x) = s((s($x) minus s($x)) divide s($x)) "A"
s($x) divide s($x) = s((s($(x) minus s($x)) divide s($x)) "B"
if s($x) ge s($x) = true then s($x) divide s($x) = ( (s($x) minus s($x)) divide s($x) ) ~ s( zero divide s($x) ) "C"
s( zero divide s($x) ) "D"
if ge(zero,s($x)) = false then zero divide s($x) = zero; "F"
zero divide s($x) = zero; "G"

s(zero divide s($x) )= s( zero ) "H"

\end{filecontents*}